.

HumanProof/Meta/BinTree.lean
@@ -7,16 +7,18 @@ inductive BinTree (α : Type u) where
 | leaf : α → BinTree α
 | node : Nat → BinTree α → BinTree α → BinTree α
 
+namespace BinTree
+
 variable {α : Type u}
 
-def BinTree.get (tree : BinTree α) (n : Nat) : α :=
+def get (tree : BinTree α) (n : Nat) : α :=
   match tree with
   | leaf a => a
   | node m l r => if n < m then l.get n else r.get n
 
 open Lean Qq
 
-def BinTree.mkExpr {u : Level} {α : Q(Type $u)} (atoms : Array Q($α)) : Q(BinTree $α) :=
+def mkExpr {u : Level} {α : Q(Type $u)} (atoms : Array Q($α)) : Q(BinTree $α) :=
   if _ : atoms.size = 0 then
     panic! "empty array"
   else
@@ -33,6 +35,131 @@ where
       q(node $n $l $r)
   termination_by hi - lo
 
-def BinTree.mkFun {u : Level} {α : Q(Type $u)} (atoms : Array Q($α)) : Q(Nat → $α) :=
+def mkFun {u : Level} {α : Q(Type $u)} (atoms : Array Q($α)) : Q(Nat → $α) :=
   let tree := BinTree.mkExpr atoms
   q(($tree).get)
+
+
+/-
+The avobe is sufficient to use `BinTree` purely as an lookup index expression
+However, we may also like to use it as an index that is created and modifies by the kernel.
+
+Thus, we introduce more operations, such as a boolean equality, and modification.
+-/
+
+def modify (f : α → α) (n : Nat) : BinTree α → BinTree α
+| .leaf a     => .leaf (f a)
+| .node m l r => if n < m then .node m (l.modify f n) r else .node m l (r.modify f n)
+
+def beq [BEq α] : BinTree α → BinTree α → Bool
+| .leaf a, .leaf b => a == b
+| .node _ l r, .node _ l' r' => Bool.and (beq l l') (beq r r')
+| _, _ => false
+
+
+inductive Equiv : BinTree α → BinTree α → Prop where
+| leaf (a b : α)            : Equiv (.leaf a) (.leaf b)
+| node (m : Nat) (l l' r r' : BinTree α) : Equiv l l' → Equiv r r' → Equiv (.node m l r) (.node m l' r')
+
+
+theorem trans (t₁ t₂ t₃ : BinTree α) (h : t₁.Equiv t₂) (h' : t₂.Equiv t₃) : t₁.Equiv t₃ := by
+  induction t₁ generalizing t₂ t₃ with
+  | leaf a => cases h with
+    | leaf _ b => cases h' with
+      | leaf _ c => exact Equiv.leaf a c
+  | node m l r ih_l ih_r => cases h with
+    | node _ _ l' _ r' h'' h''' => cases h' with
+      | node _ _ l'' _ r'' h'''' h''''' =>
+        exact Equiv.node m l l'' r r'' (ih_l l' l'' h'' h'''') (ih_r r' r'' h''' h''''')
+
+theorem symm (t₁ t₂ : BinTree α) (h : t₁.Equiv t₂) : t₂.Equiv t₁ := by
+  induction t₁ generalizing t₂ with
+  | leaf a => cases t₂ with
+    | leaf b => exact Equiv.leaf b a
+    | node => contradiction
+  | node m l r ih_l ih_r =>
+    cases h with
+    | node _ _ l' _ r' h h' => exact Equiv.node m l' l r' r (ih_l l' h) (ih_r r' h')
+
+theorem refl (t : BinTree α) : t.Equiv t := by
+  induction t with
+  | leaf a => exact Equiv.leaf a a
+  | node m l r ih_l ih_r => exact Equiv.node m l l r r ih_l ih_r
+
+theorem equiv_modify (f : α → α) (n : Nat) (t : BinTree α) : t.Equiv (t.modify f n) := by
+  induction t with
+  | leaf a => apply Equiv.leaf
+  | node m l r ih_l ih_r =>
+    by_cases h : n < m <;> simp [modify, h] <;> apply Equiv.node <;> first | assumption | apply refl
+
+
+inductive WF : Nat → Nat → BinTree α → Prop where
+| leaf (n : Nat) (a : α) : WF n (n+1) (.leaf a)
+| node (x y z : Nat) (l r : BinTree α) : x < y → y < z → WF x y l → WF y z r → WF x z (.node y l r)
+
+abbrev btw (x n y : Nat) := x ≤ n ∧ n < y
+
+theorem WF_modify (f : α → α) (n x y : Nat) (t : BinTree α) (h : WF x y t) : WF x y (t.modify f n) := by
+  induction t generalizing x y with
+  | leaf a => cases h with
+    | leaf n b => exact WF.leaf x (f a)
+  | node m l r ih_l ih_r => cases h with
+    | node x y z _ _ xy yz hl hr =>
+      unfold modify
+      split <;> apply WF.node <;> try assumption
+      exact ih_l x m hl
+      exact ih_r m y hr
+
+
+theorem get_modify (f : α → α) (n n' x y : Nat) (t : BinTree α) (ht : WF x y t) (hn : btw x n y) (hn' : btw x n' y) :
+    (t.modify f n').get n = if n = n' then f (t.get n) else t.get n := by
+  by_cases h : n = n' <;> simp [h]
+  · induction t generalizing x y with
+    | leaf a => cases ht with
+      | leaf _ _ =>
+        obtain rfl : x = n := by omega
+        obtain rfl : x = n' := by omega
+        unfold modify get
+        rfl
+    | node m l r ih_l ih_r => cases ht with
+      | node x y z _ _ xy yz hl hr =>
+        unfold modify
+        by_cases h : n' < m <;> by_cases h' : n < m <;> (try omega) <;> simp only [h, ↓reduceIte, get]
+        · apply ih_l x m <;> simp_all [btw]
+        · apply ih_r m y <;> simp_all [btw]
+  · induction t generalizing x y with
+    | leaf a => cases ht with | leaf _ _ => omega
+    | node m l r ih_l ih_r => cases ht with
+      | node x y z _ _ xy yz hl hr =>
+        unfold modify
+        by_cases h : n' < m <;> by_cases h' : n < m <;> simp only [h, ↓reduceIte, get, h']
+        · apply ih_l x m <;> simp_all [btw]
+        · apply ih_r m y <;> simp_all [btw]
+
+def initial (lo hi fuel : Nat) (a : α) : BinTree α :=
+  if lo = ((lo + hi)/2) then
+    .leaf a
+  else
+    match fuel with
+    | 0 => .leaf a
+    | fuel+1 => .node ((lo + hi)/2) (initial lo ((lo + hi)/2) fuel a) (initial ((lo + hi)/2) hi fuel a)
+
+theorem WF_initial (lo hi fuel : Nat) (a : α) (h_bound : lo < hi) (h_fuel : hi ≤ lo + fuel) : WF lo hi (initial lo hi fuel a) := by
+  unfold initial
+  split
+  · obtain rfl : hi = lo+1 := by omega
+    apply WF.leaf
+  match fuel with
+  | 0 => omega
+  | fuel+1 =>
+    dsimp only
+    apply WF.node _ _ _ _ _ (by omega) (by omega)
+      <;> apply WF_initial <;> omega
+
+theorem get_initial (n lo hi fuel : Nat) (a : α) : (initial lo hi fuel a).get n = a := by
+  induction fuel generalizing lo hi with
+  | zero => simp [initial, get]
+  | succ fuel ih =>
+    simp [initial]
+    split <;> simp [get]
+    split <;> apply ih
